Lectures/Week08/Sheet2.lean
@@ -26,19 +26,21 @@ def merge (xs ys : List ℕ) : TimeM (List ℕ) :=
 def mergeSort (xs : List ℕ) : TimeM (List ℕ) :=  do
   if xs.length < 2 then return xs
   else
-    let n := xs.length
-    let half := n / 2
-    let left :=  xs.take half
+    let half  := xs.length / 2
+    let left  :=  xs.take half
     let right := xs.drop half
-    let sortedLeft ← mergeSort left
+    let sortedLeft  ← mergeSort left
     let sortedRight ← mergeSort right
     merge sortedLeft sortedRight
 
 -- # interpretation in each line
+
 -- If the return type is a monad, say (`List ℕ`), then
 -- `let sortedLeft ← mergeSort left`
--- This line means you can treat `sortedLeft` as type List ℕ and let notation tell Lean to put `sortedLeft` into a box
--- If the return type is not a monad, you can use normal `let` with `:=` notation.
+
+-- This line means you can treat `sortedLeft` as type List ℕ and let notation
+-- tell Lean to put `sortedLeft` into a box If the return type is not a monad,
+-- you can use normal `let` with `:=` notation.
 
 
 #check mergeSort
@@ -47,16 +49,17 @@ def mergeSort (xs : List ℕ) : TimeM (List ℕ) :=  do
 
 -- Correctness of Merge sort
 
-@[simp,grind] def Nat.MinOfList (a :ℕ ) (t: List ℕ) : Prop := ∀ y ∈ t, a ≤ y
+@[simp,grind] def Nat.MinOfList (a : ℕ) (t : List ℕ) : Prop := ∀ y ∈ t, a ≤ y
 
 -- inductive predicate
 inductive Sorted: List ℕ  → Prop
   | nil : Sorted []
   | single (a : ℕ) : Sorted [a]
-  | cons (a b : ℕ) (t : List ℕ ) : a ≤ b → Sorted (b :: t) → Sorted (a :: b :: t)
-  | cons_min (a :ℕ) (t : List ℕ) : a.MinOfList t → Sorted (t) →  Sorted (a :: t)
+  | cons (a b : ℕ) (t : List ℕ) : a ≤ b → Sorted (b :: t) → Sorted (a :: b :: t)
+  | cons_min (a : ℕ) (t : List ℕ) : a.MinOfList t → Sorted t →  Sorted (a :: t)
 
-theorem sorted_min {x : ℕ} {xs : List ℕ} (hxs : Sorted (x :: xs)) :  x.MinOfList xs  := by
+theorem sorted_min {x : ℕ} {xs : List ℕ} (hxs : Sorted (x :: xs))
+  : x.MinOfList xs := by
   cases hxs
   · simp
   · simp only [Nat.MinOfList, List.mem_cons, forall_eq_or_imp]
@@ -66,21 +69,97 @@ theorem sorted_min {x : ℕ} {xs : List ℕ} (hxs : Sorted (x :: xs)) :  x.MinOf
       grind
   · exact a_1
 
-theorem sorted_is_preserved_by_min_cons {a : ℕ} {t : List ℕ} (hmin : a.MinOfList t) (ht : Sorted t) : Sorted (a :: t) := by
+theorem sorted_is_preserved_by_min_cons {a : ℕ} {t : List ℕ}
+  (hmin : a.MinOfList t) (ht : Sorted t) : Sorted (a :: t) := by
   exact Sorted.cons_min a t hmin ht
 
-theorem sorted_suffix {x : ℕ} {xs : List ℕ} (hxs : Sorted (x :: xs)) : Sorted xs := sorry
+theorem sorted_suffix {x : ℕ} {xs : List ℕ} (hxs : Sorted (x :: xs))
+  : Sorted xs := by
+  cases hxs
+  . exact Sorted.nil
+  . assumption
+  . assumption
 
--- Exercise: Port your the proof of merge sort in the previous lectures into this proof.
+
+-- Exercise: Port your the proof of merge sort in the previous lectures into
+-- this proof.
 
 theorem mem_either_merge (xs ys : List ℕ) (z : ℕ)
-  (hz : z ∈ (merge xs ys).ret) : z ∈ xs ∨ z ∈ ys := by sorry
+  (hz : z ∈ (merge xs ys).ret) : z ∈ xs ∨ z ∈ ys := by
+  induction' xs with a as ih generalizing ys
+  . simp [merge, merge.go] at hz
+    right
+    assumption
+  . simp [merge] at hz
+    induction' ys with b bs ih₂
+    . left
+      simp [merge.go] at hz
+      grind
+    . by_cases h : a ≤ b
+      . unfold merge.go at hz
+        simp [h] at hz
+        cases hz
+        . grind
+        . grind [merge]
+      . unfold merge.go at hz
+        simp [h] at hz
+        cases hz
+        . grind
+        . grind
+
 
 theorem min_all_merge (x : ℕ) (xs ys : List ℕ)
-(hxs : x.MinOfList xs) (hys : x.MinOfList ys) : x.MinOfList (merge xs ys).ret := by sorry
+ (hxs : x.MinOfList xs) (hys : x.MinOfList ys)
+ : x.MinOfList (merge xs ys).ret := by
+ simp
+ intro z hz
+ have h : z ∈ xs ∨ z ∈ ys := by
+   exact mem_either_merge xs ys z hz
+ obtain h1 | h2 := h
+ . exact hxs z h1
+ . exact hys z h2
+
 
 theorem sorted_merge {l1 l2 : List ℕ} (hxs : Sorted l1)
-  (hys : Sorted l2) : Sorted ((merge l1 l2).ret) := by sorry
+  (hys : Sorted l2) : Sorted ((merge l1 l2).ret) := by
+  match l1,l2 with
+  | [], xs =>
+    simp [merge, merge.go]; assumption
+  | xs, [] =>
+    simp [merge]
+    cases xs
+    all_goals simp [merge.go]; assumption
+  | x::xs, y::ys =>
+    simp [merge, merge.go]
+    split_ifs with h
+    · apply Sorted.cons_min
+      apply sorted_min at hxs
+      apply sorted_min at hys
+      · apply min_all_merge
+        · grind
+        · grind
+      · apply sorted_merge
+        · exact sorted_suffix hxs
+        · exact hys
+    · apply Sorted.cons_min
+      apply sorted_min at hxs
+      apply sorted_min at hys
+      · apply min_all_merge
+        · grind
+        · grind
+      · apply sorted_merge
+        · exact hxs
+        · exact sorted_suffix hys
 
 -- Let's do this one as an example.
-theorem MSMCorrect (xs : List ℕ) : Sorted (mergeSort xs).ret := by sorry
+theorem MSMCorrect (xs : List ℕ)
+  : Sorted (mergeSort xs).ret := by
+  induction xs using mergeSort.induct
+  . simp [mergeSort, h]
+    cases x
+    . exact Sorted.nil
+    . simp at h
+      rw [h]
+      exact Sorted.single head
+  . rw [mergeSort]; simp [h]
+    exact sorted_merge ih2 ih1
